# Q1
## a
$$\phi_1 = (((A ∨ (B → C)) ∧ (¬C ∨ D)) → ((A → D) ∨ (C ↔ E)))$$
**Conclusion:**
satisfiable

**Justification:**
if `A = true, D = true`, then the implication holds
if `A = true, D = false, C = false, E =true`, then the implication fails

$$\phi_2 = $$
**Conclusion:**

**Justification:**

$$\phi_3 = $$
**Conclusion:**

**Justification:**

---
## b

---
## c

---
### i

---
### ii

---
# Q2
## Q2.1

---
## Q2.2

---
## Q2.3

---
## Q2.4

---
# Q3
## a

---
## b

---
## c
### i
### ii

---
## d


